lakefile.lean
@@ -3,11 +3,12 @@ open Lake DSL
 
 package «PlutusCore» where
   -- add package configuration options here
-  require Blaster from git "https://github.com/input-output-hk/Lean-blaster" @ "main"
+  require Blaster from git "https://github.com/input-output-hk/Lean-blaster" @ "beta-lambda-cache-optimization"
 
 @[default_target]
 lean_lib «PlutusCore» where
-  -- add library configuration options here
+  precompileModules := true
+  moreLeancArgs := #["-O3"]
 
 @[test_driver]
 lean_lib «Tests» where
